SMT/Reasoning/LooseningDefs.lean
@@ -1,0 +1,1003 @@
+import Encoder.Loosening
+import SMT.Reasoning.Defs
+import SMT.Reasoning.Lemmas
+
+set_option linter.style.nameCheck false
+
+open Std.Do SMT ZFSet
+
+namespace ShapeForcing
+
+/- Base sorts only cast to themselves. -/
+@[simp] lemma unit_cast_true_iff  {β} :
+  ((SMTType.unit ⊑ β) = true) ↔ β = .unit := by
+  cases β <;> simp [castable?]
+@[simp] lemma cast_unit_true_iff'  {β} :
+  ((β ⊑ SMTType.unit) = true) ↔ β = .unit := by
+  cases β <;> simp [castable?]
+
+@[simp] lemma int_cast_true_iff   {β} :
+  ((SMTType.int  ⊑ β) = true) ↔ β = .int := by
+  cases β <;> simp [castable?]
+@[simp] lemma cast_int_true_iff   {β} :
+  ((β ⊑ SMTType.int) = true) ↔ β = .int := by
+  cases β <;> simp [castable?]
+
+@[simp] lemma bool_cast_true_iff  {β} :
+  ((SMTType.bool ⊑ β) = true) ↔ β = .bool := by
+  cases β <;> simp [castable?]
+@[simp] lemma cast_bool_true_iff  {β} :
+  ((β ⊑ SMTType.bool) = true) ↔ β = .bool := by
+  cases β <;> simp [castable?]
+
+/- Pairs only cast to pairs, componentwise. -/
+
+@[simp] lemma pair_cast_true_iff {α₁ α₂ β} :
+  (((.pair α₁ α₂) ⊑ β) = true) ↔
+    ∃ β₁ β₂, β = .pair β₁ β₂ ∧ (α₁ ⊑ β₁) = true ∧ (α₂ ⊑ β₂) = true := by
+  cases β <;> simp [castable?, Bool.and_eq_true]
+@[simp] lemma cast_pair_true_iff {α₁ α₂ β} :
+  ((β ⊑ (.pair α₁ α₂)) = true) ↔
+    ∃ β₁ β₂, β = .pair β₁ β₂ ∧ (β₁ ⊑ α₁) = true ∧ (β₂ ⊑ α₂) = true := by
+  cases β <;> simp [castable?, Bool.and_eq_true]
+
+/- Options only cast to options, pointwise. -/
+
+@[simp] lemma option_cast_true_iff {α β} :
+  (((.option α) ⊑ β) = true) ↔ ∃ β', β = .option β' ∧ (α ⊑ β') = true := by
+  cases β <;> simp [castable?]
+@[simp] lemma cast_option_true_iff {α β} :
+  ((β ⊑ (.option α)) = true) ↔ ∃ β', β = .option β' ∧ (β' ⊑ α) = true := by
+  cases β <;> simp [castable?]
+
+/- Predicates are covariant in the domain. -/
+@[simp] lemma fun_bool_cast_true_iff {α β} :
+  (((.fun α .bool) ⊑ β) = true) ↔ ∃ α', β = .fun α' .bool ∧ (α ⊑ α') = true := by
+  induction β <;> simp [castable?]
+  case «fun» τ σ τ_ih σ_ih =>
+    iff_rintro h ⟨rfl, h⟩
+    · cases σ with
+      | bool =>
+        unfold castable? at h
+        split at h <;> injections <;>
+        · subst_vars
+          exact ⟨rfl, h⟩
+      | unit | «fun» | option | pair | int => simp only [castable?, Bool.false_eq_true] at h
+    · unfold castable?
+      split <;> injections
+      · subst_vars
+        exact h
+      · subst_vars
+        exact h
+      · rename_i contr _ _ _ _ _
+        nomatch contr α τ rfl rfl
+
+@[simp] lemma cast_fun_bool_true_iff {α β} :
+  ((β ⊑ (.fun α .bool)) = true) ↔
+    (∃ α', β = .fun α' .bool ∧ (α' ⊑ α) = true) ∨
+    (∃ α' β' α'' β'', β = .fun α' (.option β') ∧ α = .pair α'' β'' ∧ (α' ⊑ α'') = true ∧ (β' ⊑ β'') = true) := by
+  induction β generalizing α
+  case «fun» τ σ τ_ih σ_ih =>
+    iff_rintro h ( ⟨_, ⟨⟩, h⟩ | ⟨α', β', α'', β'', ⟨⟩, rfl, τ_α'', σ_β''⟩ )
+    · cases σ with
+      | bool =>
+        simp only [fun_bool_cast_true_iff, SMTType.fun.injEq, and_true, exists_eq_left'] at h
+        left
+        use τ
+      | pair | int | unit | «fun» => simp only [castable?, Bool.false_eq_true] at h
+      | option σ =>
+        unfold castable? at h
+        split at h <;> injections
+        subst_eqs
+        rw [Bool.and_eq_true] at h
+        rename_i δ γ
+        right
+        use τ, σ, δ, γ
+    · simpa only [fun_bool_cast_true_iff, SMTType.fun.injEq, and_true, exists_eq_left']
+    · unfold castable?
+      simp only [Bool.and_eq_true]
+      exact ⟨τ_α'', σ_β''⟩
+  all_goals simp only [castable?, Bool.false_eq_true, reduceCtorEq, false_and, exists_const, or_self]
+
+/- Option-valued functions: either widen to another option-valued function or view as its graph predicate over pairs. -/
+@[simp] lemma fun_opt_cast_true_iff {α β γ} :
+  (((.fun α (.option β)) ⊑ γ) = true) ↔
+    (∃ α' β', γ = .fun α' (.option β') ∧ (α ⊑ α') = true ∧ (β ⊑ β') = true) ∨
+    (∃ α' β', γ = .fun (.pair α' β') .bool ∧ (α ⊑ α') = true ∧ (β ⊑ β') = true) := by
+  induction γ generalizing α β <;> simp [castable?]
+  case «fun» τ σ τ_ih σ_ih =>
+    iff_rintro h (⟨α', rfl, α_τ, β_α'⟩ | ⟨α', β', ⟨rfl, rfl⟩, α_α', β_β'⟩ )
+    · cases σ with
+      | «fun» | pair | unit | int => simp only [castable?, Bool.false_eq_true] at h
+      | bool =>
+        unfold castable? at h
+        split at h <;> injections
+        subst_vars
+        rename_i _ _ δ γ
+        rw [Bool.and_eq_true] at h
+        right
+        use δ, γ
+      | option σ =>
+        left
+        simp only [castable?, Bool.and_eq_true] at h
+        use σ
+    · unfold castable?
+      simp only [Bool.and_eq_true]
+      exact ⟨α_τ, β_α'⟩
+    · unfold castable?
+      simp only [Bool.and_eq_true]
+      exact ⟨α_α', β_β'⟩
+@[simp] lemma cast_fun_opt_true_iff {α β γ} :
+  ((γ ⊑ (.fun α (.option β))) = true) ↔
+    (∃ α' β', γ = .fun α' (.option β') ∧ (α' ⊑ α) = true ∧ (β' ⊑ β) = true) := by
+  induction γ generalizing α β <;> simp [castable?]
+  case «fun» τ σ τ_ih σ_ih =>
+    iff_rintro h ⟨α', rfl, α_τ, α'_β⟩
+    · cases σ with
+      | bool | «fun» | pair | unit | int => simp only [castable?, Bool.false_eq_true] at h
+      | option σ =>
+        simp only [fun_opt_cast_true_iff, SMTType.fun.injEq, SMTType.option.injEq, existsAndEq,
+          and_true, exists_eq_left', reduceCtorEq, and_false, false_and, exists_const,
+          or_false] at h
+        use σ
+    · simp only [fun_opt_cast_true_iff, SMTType.fun.injEq, SMTType.option.injEq, existsAndEq,
+        and_true, exists_eq_left', reduceCtorEq, and_false, false_and, exists_const, or_false]
+      exact ⟨α_τ, α'_β⟩
+
+/-- Pair → Bool predicates -/
+@[simp] lemma pairPred_cast_true_iff {α β γ} :
+  (((.fun (.pair α β) .bool) ⊑ γ) = true) ↔
+    ∃ α' β', γ = .fun (.pair α' β') .bool ∧ (α ⊑ α') = true ∧ (β ⊑ β') = true := by
+  induction γ generalizing α β <;> simp [castable?]
+  case «fun» τ σ τ_ih σ_ih =>
+    iff_rintro h ⟨α', β', ⟨rfl, rfl⟩, α_α', β_β'⟩
+    · cases σ with
+      | bool =>
+        obtain ⟨-, β₁, β₂, rfl, α_β₁, β_β₂⟩ := h
+        use β₁, β₂
+      | int | unit | «fun» | option | pair => nomatch h.1
+    · exact ⟨rfl, α', β', rfl, α_α', β_β'⟩
+@[simp] lemma cast_pairPred_true_iff {α β γ} :
+  ((γ ⊑ (.fun (.pair α β) .bool)) = true) ↔
+    (∃ α' β', γ = .fun (.pair α' β') .bool ∧ (α' ⊑ α) = true ∧ (β' ⊑ β) = true) ∨
+    (∃ α' β', γ = .fun α' (.option β') ∧ (α' ⊑ α) = true ∧ (β' ⊑ β) = true) := by
+  induction γ generalizing α β <;> simp [castable?]
+  case «fun» τ σ τ_ih σ_ih =>
+    iff_rintro h ( ⟨α', β', ⟨rfl, rfl⟩, α_α', β_β'⟩ | ⟨α', rfl, τ_α, α'_β⟩ )
+    · cases σ with
+      | bool =>
+        simp only [true_and, reduceCtorEq, false_and, exists_const, or_false, and_true] at h ⊢
+        exact h
+      | «fun» | int | unit | pair => simp only [reduceCtorEq, false_and, exists_const, or_self] at h
+      | option σ =>
+        simp only [reduceCtorEq, false_and, SMTType.option.injEq,
+          exists_eq_left', false_or, and_false, exists_const] at h ⊢
+        exact h
+    · simp only [SMTType.pair.injEq, existsAndEq, and_true, exists_eq_left', true_and,
+      reduceCtorEq, false_and, exists_const, or_false]
+      exact ⟨α_α', β_β'⟩
+    · simp only [reduceCtorEq, false_and, SMTType.option.injEq, exists_eq_left', false_or]
+      exact ⟨τ_α, α'_β⟩
+
+/-- A data certificate describing *how* `α` casts to `β`. -/
+inductive CastPath : SMTType → SMTType → Type
+| unit  : CastPath .unit .unit
+| int   : CastPath .int  .int
+| bool  : CastPath .bool .bool
+| pair {a₁ a₂ b₁ b₂} (p₁ : CastPath a₁ b₁) (p₂ : CastPath a₂ b₂) :
+  CastPath (.pair a₁ a₂) (.pair b₁ b₂)
+| option {a b} (p : CastPath a b) :
+  CastPath (.option a) (.option b)
+| funBool {a a'} (p : CastPath a a') :
+    CastPath (.fun a .bool) (.fun a' .bool)
+| funOpt_fun {a a' b b'} (pd : CastPath a a') (pc : CastPath b b') :
+    CastPath (.fun a (.option b)) (.fun a' (.option b'))
+| funOpt_graph {a a' b b'} (pd : CastPath a a') (pc : CastPath b b') :
+    CastPath (.fun a (.option b)) (.fun (.pair a' b') .bool)
+| pairPred {a a' b b'} (p₁ : CastPath a a') (p₂ : CastPath b b') :
+    CastPath (.fun (.pair a b) .bool) (.fun (.pair a' b') .bool)
+  deriving BEq, DecidableEq
+
+end ShapeForcing
+
+open ShapeForcing
+
+/-- Build a `CastPath α β` from a truth witness `(α ⊑ β) = true` -/
+noncomputable def CastPath.of_true (α β : SMTType) (h : (α ⊑ β) = true) :
+    CastPath α β :=
+  match hα : α with
+  | .unit => by
+      subst hα
+      have : β = .unit := unit_cast_true_iff.mp h
+      exact this ▸ CastPath.unit
+  | .int => by
+      subst hα
+      have : β = .int := int_cast_true_iff.mp h
+      exact this ▸ CastPath.int
+  | .bool => by
+      subst hα
+      have : β = .bool := bool_cast_true_iff.mp h
+      exact this ▸ CastPath.bool
+  | .pair a₁ a₂ => by
+      subst hα
+      -- shape forcing gives us β₁, β₂ and recursive witnesses
+      choose β₁ β₂ hβ h₁ h₂ using (pair_cast_true_iff).mp h
+      subst hβ
+      exact CastPath.pair (CastPath.of_true a₁ β₁ h₁) (CastPath.of_true a₂ β₂ h₂)
+  | .option a => by
+      subst hα
+      choose β' hβ ha using (option_cast_true_iff).mp h
+      subst hβ
+      exact CastPath.option (CastPath.of_true a β' ha)
+  | .fun (.pair a b) .bool => by
+      subst hα
+      choose a' b' hγ ha hb using (pairPred_cast_true_iff).mp h
+      subst hγ
+      exact CastPath.pairPred (CastPath.of_true a a' ha) (CastPath.of_true b b' hb)
+  | .fun a .bool => by
+      subst hα
+      choose a' ha hdom using (fun_bool_cast_true_iff).mp h
+      subst ha
+      exact CastPath.funBool (CastPath.of_true a a' hdom)
+  | .fun a (.option b) => by
+      subst hα
+      let cases := (fun_opt_cast_true_iff).mp h
+      if hcases : ∃ α' β', β = α'.fun β'.option ∧ a ⊑ α' = true ∧ b ⊑ β' = true then
+        choose a' b' hγ ha hb using hcases
+        subst hγ
+        exact CastPath.funOpt_fun (CastPath.of_true a a' ha) (CastPath.of_true b b' hb)
+      else
+        choose a' b' hγ ha hb using Or.resolve_left cases hcases
+        subst hγ
+        exact CastPath.funOpt_graph (CastPath.of_true a a' ha) (CastPath.of_true b b' hb)
+  | SMTType.fun (SMTType.pair _ _) (SMTType.pair _ _)
+  | SMTType.fun (SMTType.pair _ _) (SMTType.fun _ _)
+  | SMTType.fun (SMTType.pair _ _) SMTType.unit
+  | SMTType.fun (SMTType.pair _ _) SMTType.int
+  | SMTType.fun (SMTType.option _) (SMTType.pair _ _)
+  | SMTType.fun (SMTType.option _) (SMTType.fun _ _)
+  | SMTType.fun (SMTType.option _) SMTType.unit
+  | SMTType.fun (SMTType.option _) SMTType.int
+  | SMTType.fun (SMTType.fun _ _) (SMTType.pair _ _)
+  | SMTType.fun (SMTType.fun _ _) (SMTType.fun _ _)
+  | SMTType.fun (SMTType.fun _ _) SMTType.unit
+  | SMTType.fun (SMTType.fun _ _) SMTType.int
+  | SMTType.fun SMTType.unit (SMTType.pair _ _)
+  | SMTType.fun SMTType.unit (SMTType.fun _ _)
+  | SMTType.fun SMTType.unit SMTType.unit
+  | SMTType.fun SMTType.unit SMTType.int
+  | SMTType.fun SMTType.int (SMTType.pair _ _)
+  | SMTType.fun SMTType.int (SMTType.fun _ _)
+  | SMTType.fun SMTType.int SMTType.unit
+  | SMTType.fun SMTType.int SMTType.int
+  | SMTType.fun SMTType.bool (SMTType.pair _ _)
+  | SMTType.fun SMTType.bool (SMTType.fun _ _)
+  | SMTType.fun SMTType.bool SMTType.unit
+  | SMTType.fun SMTType.bool SMTType.int => by
+    subst hα
+    simp only [castable?, Bool.false_eq_true] at h
+
+noncomputable section CastPathToZF
+open Classical
+
+abbrev castZF_pair {α₁ β₁ α₂ β₂ : SMTType} :
+  {ζ₁ // IsFunc ⟦α₁⟧ᶻ ⟦β₁⟧ᶻ ζ₁} →
+  {ζ₂ // IsFunc ⟦α₂⟧ᶻ ⟦β₂⟧ᶻ ζ₂} →
+  {f : ZFSet // IsFunc ⟦.pair α₁ α₂⟧ᶻ ⟦.pair β₁ β₂⟧ᶻ f} :=
+  fun ⟨ζ₁, hζ₁⟩ ⟨ζ₂, hζ₂⟩ ↦ ⟨fprod ζ₁ ζ₂, ZFSet.fprod_is_func hζ₁ hζ₂⟩
+
+abbrev castZF_option {α β : SMTType} :
+  {ζ // IsFunc ⟦α⟧ᶻ ⟦β⟧ᶻ ζ} →
+  {f : ZFSet // IsFunc ⟦α.option⟧ᶻ ⟦β.option⟧ᶻ f} := fun ⟨ζ, hζ⟩ ↦
+  let fopt : ZFSet :=
+    λᶻ: ⟦α.option⟧ᶻ → ⟦β.option⟧ᶻ
+      |     x       ↦ if hx : x ∈ ⟦α.option⟧ᶻ then
+                        if is_none : x = ZFSet.Option.none (S := ⟦α⟧ᶻ).val then
+                          ZFSet.Option.none (S := ⟦β⟧ᶻ).val
+                        else
+                          have y_def : ∃ y, x = (ZFSet.Option.some (S := ⟦α⟧ᶻ) y).val := by
+                            obtain ⟨y, hy⟩ := ZFSet.Option.casesOn ⟨x, hx⟩ |>.resolve_left (by rw [Subtype.ext_iff]; exact
+                              is_none)
+                            rw [Subtype.ext_iff] at hy
+                            use y
+                          let ⟨y, hy⟩ := Classical.choose y_def
+                          ZFSet.Option.some (S := ⟦β⟧ᶻ) (@ᶻζ ⟨y, by rwa [ZFSet.is_func_dom_eq]⟩) |>.val
+                      else ∅
+  have hfopt : IsFunc ⟦α.option⟧ᶻ ⟦β.option⟧ᶻ fopt := by
+    apply ZFSet.lambda_isFunc
+    intro x hx
+    rw [dite_cond_eq_true (eq_true hx)]
+    split_ifs with is_none <;> apply SetLike.coe_mem
+  ⟨fopt, hfopt⟩
+
+abbrev castZF_funBool {α β : SMTType} :
+  {f // IsFunc ⟦α⟧ᶻ ⟦β⟧ᶻ f} →
+  {ff : ZFSet // IsFunc ⟦.fun α .bool⟧ᶻ ⟦.fun β .bool⟧ᶻ ff} :=
+  fun ⟨cast, hcast⟩ ↦
+    let ff : ZFSet :=
+      λᶻ: ⟦.fun α .bool⟧ᶻ → ⟦.fun β .bool⟧ᶻ
+        |     f_α          ↦ if hf_α : IsFunc ⟦α⟧ᶻ 𝔹 f_α then
+                              λᶻ: ⟦β⟧ᶻ → .𝔹
+                                |   y  ↦ if y_ran : y ∈ cast.Range then
+                                            let x := choose (mem_sep.mp y_ran).2
+                                            have hx : x ∈ ⟦α⟧ᶻ := by
+                                              have ⟨dom, _⟩ := choose_spec (mem_sep.mp y_ran).2
+                                              conv at dom =>
+                                                enter [1]
+                                                rw [is_func_dom_eq]
+                                              exact dom
+                                            @ᶻf_α ⟨x, by rwa [is_func_dom_eq]⟩
+                                          else zffalse
+                            else ∅
+    have hff : IsFunc ⟦.fun α .bool⟧ᶻ ⟦.fun β .bool⟧ᶻ ff := by
+      apply lambda_isFunc
+      intro f_α hf_α
+      rw [mem_funs] at hf_α
+      rw [dite_cond_eq_true (eq_true hf_α), mem_funs]
+      apply lambda_isFunc
+      intro y hy
+      split_ifs with y_ran
+      · apply SetLike.coe_mem
+      · exact ZFBool.zffalse_mem_𝔹
+    ⟨ff, hff⟩
+
+abbrev castZF_funOpt {α₁ α₂ β₁ β₂ : SMTType} :
+  {ζ₁ // IsFunc ⟦α₁⟧ᶻ ⟦α₂⟧ᶻ ζ₁} →
+  {ζ₂ // IsFunc ⟦β₁⟧ᶻ ⟦β₂⟧ᶻ ζ₂} →
+  {ff : ZFSet // IsFunc ⟦.fun α₁ (.option β₁)⟧ᶻ ⟦.fun α₂ (.option β₂)⟧ᶻ ff} :=
+  fun ⟨ζ₁, hζ₁⟩ ⟨ζ₂, hζ₂⟩ ↦
+    let ⟨ζ₂', hζ₂'⟩ := ZFSet.Option.flift ζ₂ hζ₂
+    let ff : ZFSet :=
+      (λᶻ : ⟦.fun α₁ (.option β₁)⟧ᶻ → ⟦.fun α₂ (.option β₂)⟧ᶻ
+          |              F          ↦ if hF : IsFunc ⟦α₁⟧ᶻ ⟦.option β₁⟧ᶻ F then
+                                        -- ζ₂' ∘ᶻ (F ∘ᶻ ζ₁⁻¹)
+                                        λᶻ: ⟦α₂⟧ᶻ → ⟦.option β₂⟧ᶻ
+                                          |   x   ↦ if hx : x ∈ ζ₁.Range then
+                                                      let x' := choose (mem_sep.mp hx).2
+                                                      have hx' : x' ∈ ⟦α₁⟧ᶻ := by
+                                                        have ⟨dom, _⟩ := choose_spec (mem_sep.mp hx).2
+                                                        conv at dom =>
+                                                          enter [1]
+                                                          rw [is_func_dom_eq]
+                                                        exact dom
+                                                      let y := fapply F (is_func_is_pfunc hF) ⟨x', by rwa [is_func_dom_eq]⟩
+                                                      @ᶻζ₂' ⟨y, by rw [is_func_dom_eq]; apply Subtype.property⟩
+                                                    else ZFSet.Option.none (S := ⟦β₂⟧ᶻ).val
+                                      else ∅)
+    have hff : IsFunc ⟦.fun α₁ (.option β₁)⟧ᶻ ⟦.fun α₂ (.option β₂)⟧ᶻ ff := by
+      apply lambda_isFunc
+      intro F hF
+      rw [mem_funs] at hF
+      rw [dite_cond_eq_true (eq_true hF), mem_funs]
+      apply lambda_isFunc
+      intro y hy
+      split_ifs with hy_range <;> apply SetLike.coe_mem
+    ⟨ff, hff⟩
+
+abbrev castZF_funOpt_graph {α₁ α₂ β₁ β₂ : SMTType} :
+  {ζ₁ // IsFunc ⟦α₁⟧ᶻ ⟦α₂⟧ᶻ ζ₁} →
+  {ζ₂ // IsFunc ⟦β₁⟧ᶻ ⟦β₂⟧ᶻ ζ₂} →
+  {ff : ZFSet // IsFunc ⟦.fun α₁ (.option β₁)⟧ᶻ ⟦.fun (.pair α₂ β₂) .bool⟧ᶻ ff} :=
+  fun ⟨ζ₁, hζ₁⟩ ⟨ζ₂, hζ₂⟩ ↦
+    let R :=
+      λᶻ: ⟦.fun α₁ (.option β₁)⟧ᶻ → ⟦.fun (.pair α₂ β₂) .bool⟧ᶻ
+        | F ↦ if hF : IsFunc ⟦α₁⟧ᶻ ⟦.option β₁⟧ᶻ F then
+                λᶻ: ⟦α₂.pair β₂⟧ᶻ → .𝔹
+                  | xy ↦ if hxy : xy ∈ ⟦.pair α₂ β₂⟧ᶻ then
+                          let x := xy.π₁
+                          if x_cast : x ∈ ζ₁.Range then
+                            let x' := choose (mem_sep.mp x_cast).2
+                            have hx' : x' ∈ ⟦α₁⟧ᶻ := by
+                              have ⟨dom, _⟩ := choose_spec (mem_sep.mp x_cast).2
+                              conv at dom =>
+                                enter [1]
+                                rw [is_func_dom_eq]
+                              exact dom
+                            let y := xy.π₂
+                            if y_cast : y ∈ ζ₂.Range then
+                              let y' := choose (mem_sep.mp y_cast).2
+                              have hy' : y' ∈ ⟦β₁⟧ᶻ := by
+                                have ⟨dom, _⟩ := choose_spec (mem_sep.mp y_cast).2
+                                conv at dom =>
+                                  enter [1]
+                                  rw [is_func_dom_eq]
+                                exact dom
+                              -- now apply F to x' and see if we get some y''
+                              ZFSet.ZFBool.ofBool <|
+                                @ᶻF ⟨x', by rwa [is_func_dom_eq]⟩ = ZFSet.Option.some (S := ⟦β₁⟧ᶻ) ⟨y', hy'⟩
+                            else zffalse
+                          else zffalse
+                        else ∅
+                else ∅
+    have hR : IsFunc ⟦.fun α₁ (.option β₁)⟧ᶻ ⟦.fun (.pair α₂ β₂) .bool⟧ᶻ R := by
+      apply lambda_isFunc
+      intro F hF
+      rw [mem_funs] at hF
+      rw [dite_cond_eq_true (eq_true hF), mem_funs]
+      apply lambda_isFunc
+      intro xy hxy
+      rw [dite_cond_eq_true (eq_true hxy)]
+      dsimp
+      split_ifs
+      · apply ZFBool.mem_ofBool_𝔹
+      · exact ZFBool.zffalse_mem_𝔹
+      · exact ZFBool.zffalse_mem_𝔹
+    ⟨R, hR⟩
+
+abbrev castZF_pairPred {α₁ α₂ β₁ β₂ : SMTType} :
+  {ζ₁ // IsFunc ⟦α₁⟧ᶻ ⟦α₂⟧ᶻ ζ₁} →
+  {ζ₂ // IsFunc ⟦β₁⟧ᶻ ⟦β₂⟧ᶻ ζ₂} →
+  {ff : ZFSet // IsFunc ⟦.fun (.pair α₁ β₁) .bool⟧ᶻ ⟦.fun (.pair α₂ β₂) .bool⟧ᶻ ff} :=
+  fun ⟨ζ₁, hζ₁⟩ ⟨ζ₂, hζ₂⟩ ↦
+    let ff : ZFSet :=
+      (λᶻ : ⟦.fun (.pair α₁ β₁) .bool⟧ᶻ → ⟦.fun (.pair α₂ β₂) .bool⟧ᶻ
+          | F ↦ if hF : IsFunc ⟦.pair α₁ β₁⟧ᶻ 𝔹 F then
+                  let R :=
+                    λᶻ: ⟦α₂.pair β₂⟧ᶻ → .𝔹
+                      |       xy      ↦ if hxy : xy ∈ ⟦.pair α₂ β₂⟧ᶻ then
+                                          let x := xy.π₁
+                                          if x_cast : x ∈ ζ₁.Range then
+                                            let x' := choose (mem_sep.mp x_cast).2
+                                            have hx' : x' ∈ ⟦α₁⟧ᶻ := by
+                                              have ⟨dom, _⟩ := choose_spec (mem_sep.mp x_cast).2
+                                              conv at dom =>
+                                                enter [1]
+                                                rw [is_func_dom_eq]
+                                              exact dom
+                                            let y := xy.π₂
+                                            if y_cast : y ∈ ζ₂.Range then
+                                              let y' := choose (mem_sep.mp y_cast).2
+                                              have hy' : y' ∈ ⟦β₁⟧ᶻ := by
+                                                have ⟨dom, _⟩ := choose_spec (mem_sep.mp y_cast).2
+                                                conv at dom =>
+                                                  enter [1]
+                                                  rw [is_func_dom_eq]
+                                                exact dom
+                                                @ᶻF ⟨x'.pair y', by
+                                                  rw [is_func_dom_eq, pair_mem_prod]
+                                                  exact ⟨hx', hy'⟩⟩
+                                            else zffalse
+                                          else zffalse
+                                        else ∅
+                  R
+                else ∅)
+    have hff : IsFunc ⟦.fun (α₁.pair β₁) .bool⟧ᶻ ⟦.fun (α₂.pair β₂) .bool⟧ᶻ ff := by
+      apply lambda_isFunc
+      intro F hF
+      rw [mem_funs] at hF
+      rw [dite_cond_eq_true (eq_true hF), mem_funs]
+      apply lambda_isFunc
+      intro xy hxy
+      rw [dite_cond_eq_true (eq_true hxy)]
+      dsimp
+      split_ifs
+      · apply fapply_mem_range
+      · exact ZFBool.zffalse_mem_𝔹
+      · exact ZFBool.zffalse_mem_𝔹
+    ⟨ff, hff⟩
+
+end CastPathToZF
+
+open Classical in
+/-- Turn a `CastPath α β` into the semantic cast `⟦α⟧ᶻ → ⟦β⟧ᶻ` with an `IsFunc` certificate. -/
+noncomputable def castZF_of_path {α β : SMTType} : CastPath α β →
+  {f : ZFSet // IsFunc ⟦α⟧ᶻ ⟦β⟧ᶻ f}
+| CastPath.unit               => ⟨𝟙{∅}, Id.IsFunc⟩
+| CastPath.int                => ⟨𝟙Int, Id.IsFunc⟩
+| CastPath.bool               => ⟨𝟙𝔹, Id.IsFunc⟩
+| CastPath.pair p₁ p₂         => castZF_pair (castZF_of_path p₁) (castZF_of_path p₂)
+| CastPath.option p           => castZF_option (castZF_of_path p)
+| CastPath.funBool p          => castZF_funBool (castZF_of_path p)
+| CastPath.funOpt_fun p₁ p₂   => castZF_funOpt (castZF_of_path p₁) (castZF_of_path p₂)
+| CastPath.funOpt_graph p₁ p₂ => castZF_funOpt_graph (castZF_of_path p₁) (castZF_of_path p₂)
+| CastPath.pairPred p₁ p₂     => castZF_pairPred (castZF_of_path p₁) (castZF_of_path p₂)
+
+theorem castZF_of_path__funBool_id.{u} {α : SMTType} (hTrue : (α ⊑ α) = true)
+  (h : castZF_of_path (CastPath.of_true α α hTrue) = ⟨𝟙(SMTType.toZFSet.{u} α), Id.IsFunc⟩) :
+    castZF_funBool (castZF_of_path (CastPath.of_true α α hTrue)) =
+      ⟨𝟙(SMTType.toZFSet.{u} (.fun α .bool)), Id.IsFunc⟩ := by
+  induction α with
+  | bool | int | unit =>
+    rw [castZF_funBool]
+    congr
+    ext1 z
+    iff_rintro hz hz
+    · rw [mem_lambda] at hz
+      obtain ⟨x, y, rfl, hx, hy, rfl⟩ := hz
+      rw [mem_funs] at hx
+      rw [dite_cond_eq_true (eq_true hx)] at hy ⊢
+      rw [pair_mem_Id_iff (mem_funs.mpr hx)]
+      conv_lhs =>
+        rw [lambda_eta hx]
+      rw [lambda_ext_iff (fun hz ↦ by rw [dite_cond_eq_true (eq_true hz)]; apply Subtype.property)]
+      intro w hw
+      rw [dite_cond_eq_true (eq_true hw)]
+      split_ifs with w_ran
+      · dsimp
+        congr
+        generalize_proofs isRel exDom
+        have ⟨chs_mem, chs_spec⟩ := Classical.choose_spec exDom
+        conv at chs_spec =>
+          enter [1]
+          simp only [CastPath.of_true]
+          rw [castZF_of_path]
+          dsimp
+        rw [pair_mem_Id_iff] at chs_spec
+        · exact chs_spec.symm
+        · conv_lhs at chs_mem =>
+            rw [is_func_dom_eq]
+          exact chs_mem
+      · -- contradiction
+        conv at w_ran =>
+          enter [1,1,1]
+          simp only [CastPath.of_true]
+          rw [castZF_of_path]
+          dsimp
+        simp only [range_Id] at w_ran
+        nomatch w_ran hw
+    · rw [mem_Id_iff] at hz
+      obtain ⟨f, hf, rfl⟩ := hz
+      rw [lambda_spec]
+      refine ⟨hf, hf, ?_⟩
+      rw [mem_funs] at hf
+      rw [dite_cond_eq_true (eq_true hf)]
+      conv_lhs =>
+        rw [lambda_eta hf]
+      rw [lambda_ext_iff (fun hz ↦ by rw [dite_cond_eq_true (eq_true hz)]; apply Subtype.property)]
+      intro z hz
+      rw [dite_cond_eq_true (eq_true hz)]
+      split_ifs with z_ran
+      · dsimp
+        congr
+        generalize_proofs isRel exDom
+        have ⟨chs_mem, chs_spec⟩ := Classical.choose_spec exDom
+        conv at chs_spec =>
+          enter [1]
+          simp only [CastPath.of_true]
+          rw [castZF_of_path]
+          dsimp
+        rw [pair_mem_Id_iff] at chs_spec
+        · exact chs_spec.symm
+        · conv_lhs at chs_mem =>
+            rw [is_func_dom_eq]
+          exact chs_mem
+      · -- contradiction
+        conv at z_ran =>
+          enter [1,1,1]
+          simp only [CastPath.of_true]
+          rw [castZF_of_path]
+          dsimp
+        simp only [range_Id] at z_ran
+        nomatch z_ran hz
+  | pair α β α_ih β_ih =>
+    simp only [cast_pair_true_iff, SMTType.pair.injEq, ↓existsAndEq, and_true,
+      exists_eq_left'] at hTrue
+    obtain ⟨hα, hβ⟩ := hTrue
+    specialize α_ih hα
+    specialize β_ih hβ
+    rw [castZF_funBool]
+    congr
+    rw [ZFSet.ext_iff]
+    intro xy
+    iff_intro hxy hxy
+    · rw [mem_lambda] at hxy
+      obtain ⟨x, y, rfl, mem_x, mem_y, rfl⟩ := hxy
+      rw [mem_funs] at mem_x
+      rw [dite_cond_eq_true (eq_true mem_x)] at mem_y ⊢
+      rw [pair_mem_Id_iff (mem_funs.mpr mem_x)]
+      conv_lhs =>
+        rw [lambda_eta mem_x]
+      rw [lambda_ext_iff (fun hz ↦ by rw [dite_cond_eq_true (eq_true hz)]; apply Subtype.property)]
+      intro z hz
+      rw [dite_cond_eq_true (eq_true hz)]
+      split_ifs with z_ran
+      · dsimp
+        congr
+        generalize_proofs isRel exDom
+        have ⟨chs_mem, chs_spec⟩ := Classical.choose_spec exDom
+        simp [CastPath.of_true] at chs_spec
+
+        generalize_proofs chs₁ chs₂ hTrue₁ hTrue₂ chs_eq chs₃ at chs_spec
+
+        rw [Subtype.ext_iff] at h
+        dsimp at h
+
+        let ⟨exDom_mem, z_spec⟩ := Classical.choose_spec exDom
+        conv_lhs at z_spec =>
+          rw [h]
+        conv at exDom_mem =>
+          enter [1,1]
+          rw [h]
+        rw [is_func_dom_eq Id.IsFunc] at exDom_mem
+        symm
+        rwa [pair_mem_Id_iff exDom_mem] at z_spec
+      · -- contradiction
+        rw [Subtype.ext_iff] at h
+        dsimp at h
+        conv at z_ran =>
+          enter [1]
+          conv =>
+            enter [1,1]
+            rw [h]
+          rw [ZFSet.range_Id]
+        nomatch z_ran hz
+    · rw [mem_Id_iff] at hxy
+      obtain ⟨f, hf, rfl⟩ := hxy
+      rw [lambda_spec]
+      refine ⟨hf, hf, ?_⟩
+      rw [mem_funs] at hf
+      rw [dite_cond_eq_true (eq_true hf)]
+      conv_lhs =>
+        rw [lambda_eta hf]
+      rw [lambda_ext_iff (fun hz ↦ by rw [dite_cond_eq_true (eq_true hz)]; apply Subtype.property)]
+      intro z hz
+      rw [dite_cond_eq_true (eq_true hz)]
+      split_ifs with z_ran
+      · dsimp
+        congr
+        generalize_proofs isRel exDom
+        have ⟨chs_mem, chs_spec⟩ := Classical.choose_spec exDom
+        simp [CastPath.of_true] at chs_spec
+
+        generalize_proofs chs₁ chs₂ hTrue₁ hTrue₂ chs_eq chs₃ at chs_spec
+
+        rw [Subtype.ext_iff] at h
+        dsimp at h
+
+        let ⟨exDom_mem, z_spec⟩ := Classical.choose_spec exDom
+        conv_lhs at z_spec =>
+          rw [h]
+        conv at exDom_mem =>
+          enter [1,1]
+          rw [h]
+        rw [is_func_dom_eq Id.IsFunc] at exDom_mem
+        symm
+        rwa [pair_mem_Id_iff exDom_mem] at z_spec
+      · -- contradiction
+        rw [Subtype.ext_iff] at h
+        dsimp at h
+        conv at z_ran =>
+          enter [1]
+          conv =>
+            enter [1,1]
+            rw [h]
+          rw [ZFSet.range_Id]
+        nomatch z_ran hz
+  | option τ ih =>
+    simp only [cast_option_true_iff, SMTType.option.injEq, exists_eq_left'] at hTrue
+    specialize ih hTrue
+    rw [castZF_funBool]
+    congr
+    rw [ZFSet.ext_iff]
+    intro xy
+    iff_intro hxy hxy
+    · rw [mem_lambda] at hxy
+      obtain ⟨x, y, rfl, mem_x, mem_y, rfl⟩ := hxy
+      rw [mem_funs] at mem_x
+      rw [dite_cond_eq_true (eq_true mem_x)] at mem_y ⊢
+      rw [pair_mem_Id_iff (mem_funs.mpr mem_x)]
+      conv_lhs =>
+        rw [lambda_eta mem_x]
+      rw [lambda_ext_iff (fun hz ↦ by rw [dite_cond_eq_true (eq_true hz)]; apply Subtype.property)]
+      intro z hz
+      rw [dite_cond_eq_true (eq_true hz)]
+      split_ifs with z_ran
+      · dsimp
+        congr
+        generalize_proofs isRel exDom
+        have ⟨chs_mem, chs_spec⟩ := Classical.choose_spec exDom
+        simp [CastPath.of_true] at chs_spec
+
+        generalize_proofs chs₁ chs₂ hTrue₁ hTrue₂ chs_eq chs₃ at chs_spec
+
+        rw [Subtype.ext_iff] at h
+        dsimp at h
+
+        let ⟨exDom_mem, z_spec⟩ := Classical.choose_spec exDom
+        conv_lhs at z_spec =>
+          rw [h]
+        conv at exDom_mem =>
+          enter [1,1]
+          rw [h]
+        rw [is_func_dom_eq Id.IsFunc] at exDom_mem
+        symm
+        rwa [pair_mem_Id_iff exDom_mem] at z_spec
+      · -- contradiction
+        rw [Subtype.ext_iff] at h
+        dsimp at h
+        conv at z_ran =>
+          enter [1]
+          conv =>
+            enter [1,1]
+            rw [h]
+          rw [ZFSet.range_Id]
+        nomatch z_ran hz
+    · rw [mem_Id_iff] at hxy
+      obtain ⟨f, hf, rfl⟩ := hxy
+      rw [lambda_spec]
+      refine ⟨hf, hf, ?_⟩
+      rw [mem_funs] at hf
+      rw [dite_cond_eq_true (eq_true hf)]
+      conv_lhs =>
+        rw [lambda_eta hf]
+      rw [lambda_ext_iff (fun hz ↦ by rw [dite_cond_eq_true (eq_true hz)]; apply Subtype.property)]
+      intro z hz
+      rw [dite_cond_eq_true (eq_true hz)]
+      split_ifs with z_ran
+      · dsimp
+        congr
+        generalize_proofs isRel exDom
+        have ⟨chs_mem, chs_spec⟩ := Classical.choose_spec exDom
+        simp [CastPath.of_true] at chs_spec
+
+        generalize_proofs chs₁ chs₂ hTrue₁ hTrue₂ chs_eq chs₃ at chs_spec
+
+        rw [Subtype.ext_iff] at h
+        dsimp at h
+
+        let ⟨exDom_mem, z_spec⟩ := Classical.choose_spec exDom
+        conv_lhs at z_spec =>
+          rw [h]
+        conv at exDom_mem =>
+          enter [1,1]
+          rw [h]
+        rw [is_func_dom_eq Id.IsFunc] at exDom_mem
+        symm
+        rwa [pair_mem_Id_iff exDom_mem] at z_spec
+      · -- contradiction
+        rw [Subtype.ext_iff] at h
+        dsimp at h
+        conv at z_ran =>
+          enter [1]
+          conv =>
+            enter [1,1]
+            rw [h]
+          rw [ZFSet.range_Id]
+        nomatch z_ran hz
+  | «fun» α β α_ih β_ih =>
+    cases β with
+    | int | unit | pair α β | «fun» τ σ =>
+      simp only [castable?, Bool.false_eq_true] at hTrue
+    | option β =>
+      simp only [cast_fun_opt_true_iff, SMTType.fun.injEq, SMTType.option.injEq, ↓existsAndEq, and_true, exists_eq_left'] at hTrue
+      obtain ⟨hα, hβ⟩ := hTrue
+      specialize α_ih hα
+      specialize β_ih hβ
+      rw [castZF_funBool]
+      congr
+      rw [ZFSet.ext_iff]
+      intro xy
+      iff_intro hxy hxy
+      · rw [mem_lambda] at hxy
+        obtain ⟨x, y, rfl, mem_x, mem_y, rfl⟩ := hxy
+        rw [mem_funs] at mem_x
+        rw [dite_cond_eq_true (eq_true mem_x)] at mem_y ⊢
+        rw [pair_mem_Id_iff (mem_funs.mpr mem_x)]
+        conv_lhs =>
+          rw [lambda_eta mem_x]
+        rw [lambda_ext_iff (fun hz ↦ by rw [dite_cond_eq_true (eq_true hz)]; apply Subtype.property)]
+        intro z hz
+        rw [dite_cond_eq_true (eq_true hz)]
+        split_ifs with z_ran
+        · dsimp
+          congr
+          generalize_proofs isRel exDom
+          have ⟨chs_mem, chs_spec⟩ := Classical.choose_spec exDom
+          simp [CastPath.of_true] at chs_spec
+
+          generalize_proofs chs₁ chs₂ hTrue₁ hTrue₂ chs_eq chs₃ at chs_spec
+
+          rw [Subtype.ext_iff] at h
+          dsimp at h
+
+          let ⟨exDom_mem, z_spec⟩ := Classical.choose_spec exDom
+          conv_lhs at z_spec =>
+            rw [h]
+          conv at exDom_mem =>
+            enter [1,1]
+            rw [h]
+          rw [is_func_dom_eq Id.IsFunc] at exDom_mem
+          symm
+          rwa [pair_mem_Id_iff exDom_mem] at z_spec
+        · -- contradiction
+          rw [Subtype.ext_iff] at h
+          dsimp at h
+          conv at z_ran =>
+            enter [1]
+            conv =>
+              enter [1,1]
+              rw [h]
+            rw [ZFSet.range_Id]
+          nomatch z_ran hz
+      · rw [mem_Id_iff] at hxy
+        obtain ⟨f, hf, rfl⟩ := hxy
+        rw [lambda_spec]
+        refine ⟨hf, hf, ?_⟩
+        rw [mem_funs] at hf
+        rw [dite_cond_eq_true (eq_true hf)]
+        conv_lhs =>
+          rw [lambda_eta hf]
+        rw [lambda_ext_iff (fun hz ↦ by rw [dite_cond_eq_true (eq_true hz)]; apply Subtype.property)]
+        intro z hz
+        rw [dite_cond_eq_true (eq_true hz)]
+        split_ifs with z_ran
+        · dsimp
+          congr
+          generalize_proofs isRel exDom
+          have ⟨chs_mem, chs_spec⟩ := Classical.choose_spec exDom
+          simp [CastPath.of_true] at chs_spec
+
+          generalize_proofs chs₁ chs₂ hTrue₁ hTrue₂ chs_eq chs₃ at chs_spec
+
+          rw [Subtype.ext_iff] at h
+          dsimp at h
+
+          let ⟨exDom_mem, z_spec⟩ := Classical.choose_spec exDom
+          conv_lhs at z_spec =>
+            rw [h]
+          conv at exDom_mem =>
+            enter [1,1]
+            rw [h]
+          rw [is_func_dom_eq Id.IsFunc] at exDom_mem
+          symm
+          rwa [pair_mem_Id_iff exDom_mem] at z_spec
+        · -- contradiction
+          rw [Subtype.ext_iff] at h
+          dsimp at h
+          conv at z_ran =>
+            enter [1]
+            conv =>
+              enter [1,1]
+              rw [h]
+            rw [ZFSet.range_Id]
+          nomatch z_ran hz
+    | bool =>
+      simp only [cast_fun_bool_true_iff, SMTType.fun.injEq, and_true, exists_eq_left', reduceCtorEq, and_false, false_and, exists_const, or_false] at hTrue
+      specialize α_ih hTrue
+      rw [castZF_funBool]
+      congr
+      rw [ZFSet.ext_iff]
+      intro xy
+      iff_intro hxy hxy
+      · rw [mem_lambda] at hxy
+        obtain ⟨x, y, rfl, mem_x, mem_y, rfl⟩ := hxy
+        rw [mem_funs] at mem_x
+        rw [dite_cond_eq_true (eq_true mem_x)] at mem_y ⊢
+        rw [pair_mem_Id_iff (mem_funs.mpr mem_x)]
+        conv_lhs =>
+          rw [lambda_eta mem_x]
+        rw [lambda_ext_iff (fun hz ↦ by rw [dite_cond_eq_true (eq_true hz)]; apply Subtype.property)]
+        intro z hz
+        rw [dite_cond_eq_true (eq_true hz)]
+        split_ifs with z_ran
+        · dsimp
+          congr
+          generalize_proofs isRel exDom
+          have ⟨chs_mem, chs_spec⟩ := Classical.choose_spec exDom
+
+          generalize_proofs chs₁ chs₂ hTrue₁ hTrue₂ chs_eq chs₃ at chs_spec
+
+          rw [Subtype.ext_iff] at h
+          dsimp at h
+
+          let ⟨exDom_mem, z_spec⟩ := Classical.choose_spec exDom
+          conv_lhs at z_spec =>
+            rw [h]
+          conv at exDom_mem =>
+            enter [1,1]
+            rw [h]
+          rw [is_func_dom_eq Id.IsFunc] at exDom_mem
+          symm
+          rwa [pair_mem_Id_iff exDom_mem] at z_spec
+        · -- contradiction
+          rw [Subtype.ext_iff] at h
+          dsimp at h
+          conv at z_ran =>
+            enter [1]
+            conv =>
+              enter [1,1]
+              rw [h]
+            rw [ZFSet.range_Id]
+          nomatch z_ran hz
+      · rw [mem_Id_iff] at hxy
+        obtain ⟨f, hf, rfl⟩ := hxy
+        rw [lambda_spec]
+        refine ⟨hf, hf, ?_⟩
+        rw [mem_funs] at hf
+        rw [dite_cond_eq_true (eq_true hf)]
+        conv_lhs =>
+          rw [lambda_eta hf]
+        rw [lambda_ext_iff (fun hz ↦ by rw [dite_cond_eq_true (eq_true hz)]; apply Subtype.property)]
+        intro z hz
+        rw [dite_cond_eq_true (eq_true hz)]
+        split_ifs with z_ran
+        · dsimp
+          congr
+          generalize_proofs isRel exDom
+          have ⟨chs_mem, chs_spec⟩ := Classical.choose_spec exDom
+
+          generalize_proofs chs₁ chs₂ hTrue₁ hTrue₂ chs_eq chs₃ at chs_spec
+
+          rw [Subtype.ext_iff] at h
+          dsimp at h
+
+          let ⟨exDom_mem, z_spec⟩ := Classical.choose_spec exDom
+          conv_lhs at z_spec =>
+            rw [h]
+          conv at exDom_mem =>
+            enter [1,1]
+            rw [h]
+          rw [is_func_dom_eq Id.IsFunc] at exDom_mem
+          symm
+          rwa [pair_mem_Id_iff exDom_mem] at z_spec
+        · -- contradiction
+          rw [Subtype.ext_iff] at h
+          dsimp at h
+          conv at z_ran =>
+            enter [1]
+            conv =>
+              enter [1,1]
+              rw [h]
+            rw [ZFSet.range_Id]
+          nomatch z_ran hz
+
+lemma castZF_of_path_of_true_funBool_aux {α : SMTType} (h : (α.fun .bool ⊑ α.fun .bool) = true) :
+  castZF_of_path (CastPath.of_true (α.fun SMTType.bool) (α.fun SMTType.bool) h) =
+  castZF_funBool (castZF_of_path (CastPath.of_true α α (by simpa using h))) := by
+  conv =>
+    enter [1,1]
+    unfold CastPath.of_true
+    simp only [SMTType.fun.injEq, reduceCtorEq, and_false, false_and, exists_const, ↓reduceDIte]
+  admit
+
+
+theorem castZF_of_path_id {α : SMTType} (h : (α ⊑ α) = true) :
+    castZF_of_path (CastPath.of_true α α h) = ⟨𝟙⟦α⟧ᶻ, Id.IsFunc⟩ := by
+  induction α with
+  | bool => rfl
+  | int => rfl
+  | unit => rfl
+  | pair α β α_ih β_ih =>
+    simp only [cast_pair_true_iff, SMTType.pair.injEq, ↓existsAndEq, and_true, exists_eq_left'] at h
+    obtain ⟨hα, hβ⟩ := h
+    specialize α_ih hα
+    specialize β_ih hβ
+    rw [Subtype.ext_iff]
+    dsimp
+    ext1 xy
+    iff_intro hxy hxy
+    · rw [mem_Id_iff]
+      admit
+    · rw [mem_Id_iff] at hxy
+      obtain ⟨x, hx, rfl⟩ := hxy
+      admit
+  | «fun» α β α_ih β_ih =>
+    cases β with
+    | int | unit | pair τ σ | «fun» τ σ =>
+      simp only [castable?, Bool.false_eq_true] at h
+    | bool =>
+      have hα := h
+      simp only [cast_fun_bool_true_iff, SMTType.fun.injEq, and_true, exists_eq_left', reduceCtorEq, and_false, false_and, exists_const, or_false] at hα
+      specialize α_ih hα
+      have :
+        castZF_of_path (CastPath.of_true (α.fun SMTType.bool) (α.fun SMTType.bool) h) =
+        castZF_funBool (castZF_of_path (CastPath.of_true α α hα)) := by
+        rw [Subtype.ext_iff]
+        ext1 z
+        iff_intro hz hz
+        · simp only [mem_sep, mem_lambda, ↓existsAndEq, mem_funs, and_true]
+          admit
+        · admit
+
+      rwa [this, castZF_of_path__funBool_id hα]
+    | option β => admit
+  | option τ ih => admit
+
+
+
+open Classical in
+noncomputable def castZF.{u} (α β : SMTType) (cast? : α ⊑ β) :
+  {f : ZFSet.{u} // ⟦α⟧ᶻ.IsFunc ⟦β⟧ᶻ f} :=
+  castZF_of_path <| CastPath.of_true α β cast?
+
+-- denx! = (castZF α β cast?) @ᶻdenx ??
